% ! Tex program = xelatex
\documentclass{article}
\PassOptionsToPackage{quiet}{fontspec}% (or try silent)
% 中文
\usepackage[UTF8]{ctex}

% For more choices
% \input{/Users/anye_zhenhaoyu/Desktop/preamble.tex}
% \input{/Users/anye_zhenhaoyu/Desktop/ln_preamble.tex}

% \input{/path/preamble.tex}
% \input{/path/ln_preamble.tex}

% On my MAC's Desktop
\input{../preamble}

\graphicspath{{figures/}}

\begin{document}
% \tableofcontents
\title{\vspace{-1.5cm}Homework 3}
\maketitle

\section{Some Lemmas in Linear Algebra}
\begin{lemma}
	\[
		x^TA x=\tr(A xx^T)
	.\] 
\end{lemma}
\begin{lemma}
	\[
		\pdv{\log\abs{A}}{A}=2A^{-1}-\-{diag}(A^{-1})
		\qand
		\pdv{\tr(AB)}{A}=(B+B^T)-\-{diag}(B)
	.\] 
\end{lemma}
\section{Update $\Sigma_k$ in EM}
Now we want to find a good enough $\Sigma_k$. Our goal is to maximize the liklihood 
\[
	\+L=\sum^{N}_{n=1} \ln(\sum^{K}_{k=1} \pi_k\+N(x_n|\mu_k,\Sigma_k))
\] where 
\[
	\+N(x_n|\mu_k,\Sigma_k)
	=
	\frac{1}{\qty(2\pi)^{\flatfrac{D}{2}}\abs{\Sigma_k}^{\flatfrac{1}{2}}}
	\exp(-\frac{1}{2}(x_n-\mu_k)^T\Sigma_k^{-1}(x_n-\mu_k))
.\] 
Thus
\[
    \begin{aligned}
		\pdv{L}{A}
		&=
		\sum^{N}_{n=1} \qty{
			\frac{1}{\sum^{K}_{j=1} \pi_j\+N(x_n|\mu_j,\Sigma_j)}\times
			\pdv{A}\pi_k\+N(x_n|\mu_k,\Sigma_k)
		}
	    \\&=
		\sum^{N}_{n=1} \qty{
			\frac{\pi_k\+N(x_n|\mu_k,\Sigma_k)}{\sum^{K}_{j=1} \pi_j\+N(x_n|\mu_j,\Sigma_j)}\times
			\pdv{A}\qty[-\frac{1}{2}\log\abs{\Sigma_k}-\frac{1}{2}(x_n-\mu_k)^T\Sigma_k^{-1}(x_n-\mu_k)]
		}
		\\&=
		\sum^{N}_{n=1} \qty{
			\frac{\pi_k\+N(x_n|\mu_k,\Sigma_k)}{\sum^{K}_{j=1} \pi_j\+N(x_n|\mu_j,\Sigma_j)}\times
			\pdv{A}
			\qty[\frac{1}{2}\log\abs{\Sigma_k^{-1}}-\frac{1}{2}\tr(\Sigma_k^{-1}N_{n,k})]
		}
    \end{aligned}
.\] 
where $N_{n,k}=(x_n-\mu_k)(x_n-\mu_k)^T$. $\pdv*{L}{\Sigma_k^{-1}}=0$ gives
\[
    \sum^{N}_{n=1} \qty{
			\frac{\pi_k\+N(x_n|\mu_k,\Sigma_k)}{\sum^{K}_{j=1} \pi_j\+N(x_n|\mu_j,\Sigma_j)}\times
			\frac{1}{2}\Big[2(\Sigma_k-N_{n,k})-\-{diag}(\Sigma_k-N_{n,k})\Big]
		}=0
\] 
which entails that
\[
	\sum^{N}_{n=1} \qty[
		\frac{\pi_k\+N(x_n|\mu_k,\Sigma_k)}{\sum^{K}_{j=1} \pi_j\+N(x_n|\mu_j,\Sigma_j)}\times
		(\Sigma_k-N_{n,k})
	]=0
\] 
which entails
\[
    \Sigma_k=
	\qty(\sum^{N}_{n=1}
		\frac{\pi_k\+N(x_n|\mu_k,\Sigma_k)}{\sum^{K}_{j=1} \pi_j\+N(x_n|\mu_j,\Sigma_j)})^{-1}
	\sum^{N}_{n=1} \qty[
		\frac{\pi_k\+N(x_n|\mu_k,\Sigma_k)}{\sum^{K}_{j=1} \pi_j\+N(x_n|\mu_j,\Sigma_j)}\times
		(x_n-\mu_k)(x_n-\mu_k)^T
	]
.\] 
For simplicity, 
\[
	\gamma(z_nk)
	\defeq
	\sum^{N}_{n=1}\frac{\pi_k\+N(x_n|\mu_k,\Sigma_k)}{\sum^{K}_{j=1} \pi_j\+N(x_n|\mu_j,\Sigma_j)}
\]
Finally
\[
    \Sigma_k=
	\frac{1}{\sum^{N}_{n=1}\gamma(z_nk)}
	\sum^{N}_{n=1} \Big[
		\gamma(z_nk)(x_n-\mu_k)(x_n-\mu_k)^T
	\Big]
.\] 
Nota Bena: if we update $\mu$ first, then we could let $\mu_k$ above be  $\mu^{\-{new}}_k$.

\end{document}

